Finish refactor

LeanSorting/Basic.lean
@@ -260,196 +260,193 @@ def mergeAdjacentChunksIntoAux [Ord α] (m₁ : M₁ α) : M₁ α :=
       exact (Nat.sub_succ_lt_sub_of_lt i_lt_arr_size)
   loop m₂
 
--- theorem M₄Left.next_arr_eq
---     [Ord α]
---     {m₄Left : M₄Left α}
---     (k₁_lt_start₂ : m₄Left.k₁ < m₄Left.start₂)
---     : (m₄Left.next k₁_lt_start₂).arr = m₄Left.arr := by rfl
+theorem M₄Right.next_arr_eq
+    [Ord α]
+    {m₄Right : M₄Right α}
+    (k₂_lt_end₂ : m₄Right.k₂ < m₄Right.end₂)
+    : (m₄Right.next k₂_lt_end₂).arr = m₄Right.arr := by rfl
 
--- theorem merge_adjacent_loopLeft_arr_eq
---     [Ord α]
---     {m₄Left : M₄Left α}
---     : (mergeAdjacentChunksIntoAux.loop.loopLeft m₄Left).arr = m₄Left.arr := by
---   unfold mergeAdjacentChunksIntoAux.loop.loopLeft
---   if k₁_lt_start₂ : m₄Left.k₁ < m₄Left.start₂ then
---     simp [k₁_lt_start₂]
---     have := m₄Left.next_arr_eq
---     exact (merge_adjacent_loopLeft_arr_eq (m₄Left := m₄Left.next k₁_lt_start₂))
---   else
---     simp [k₁_lt_start₂]
--- termination_by m₄Left.start₂ - m₄Left.k₁
--- decreasing_by
---   simp_wf
---   have start₂_def : (m₄Left.next k₁_lt_start₂).start₂ = m₄Left.start₂ := by rfl
---   have k₁_def : (m₄Left.next k₁_lt_start₂).k₁ = m₄Left.k₁.succ := by rfl
---   omega
+theorem merge_adjacent_loopRight_arr_eq
+    [Ord α]
+    {m₄Right : M₄Right α}
+    : (mergeAdjacentChunksIntoAux.loop.loopLeft.loopRight m₄Right).arr = m₄Right.arr := by
+  unfold mergeAdjacentChunksIntoAux.loop.loopLeft.loopRight
+  if k₂_lt_end₂ : m₄Right.k₂ < m₄Right.end₂ then
+    simp [k₂_lt_end₂]
+    have := m₄Right.next_arr_eq
+    exact (merge_adjacent_loopRight_arr_eq (m₄Right := m₄Right.next k₂_lt_end₂))
+  else
+    simp [k₂_lt_end₂]
+termination_by m₄Right.end₂ - m₄Right.k₂
+decreasing_by
+  simp_wf
+  have end₂_def : (m₄Right.next k₂_lt_end₂).end₂ = m₄Right.end₂ := by rfl
+  have k₂_def : (m₄Right.next k₂_lt_end₂).k₂ = m₄Right.k₂.succ := by rfl
+  omega
 
--- theorem M₄Right.next_arr_eq
---     [Ord α]
---     {m₄Right : M₄Right α}
---     (k₂_lt_end₂ : m₄Right.k₂ < m₄Right.end₂)
---     : (m₄Right.next k₂_lt_end₂).arr = m₄Right.arr := by rfl
+theorem M₄Left.next_arr_eq
+    [Ord α]
+    {m₄Left : M₄Left α}
+    (k₁_lt_start₂ : m₄Left.k₁ < m₄Left.start₂)
+    : (m₄Left.next k₁_lt_start₂).arr = m₄Left.arr := by rfl
 
--- theorem merge_adjacent_loopRight_arr_eq
---     [Ord α]
---     {m₄Right : M₄Right α}
---     : (mergeAdjacentChunksIntoAux.loop.loopRight m₄Right).arr = m₄Right.arr := by
---   unfold mergeAdjacentChunksIntoAux.loop.loopRight
---   if k₂_lt_end₂ : m₄Right.k₂ < m₄Right.end₂ then
---     simp [k₂_lt_end₂]
---     have := m₄Right.next_arr_eq
---     exact (merge_adjacent_loopRight_arr_eq (m₄Right := m₄Right.next k₂_lt_end₂))
---   else
---     simp [k₂_lt_end₂]
--- termination_by m₄Right.end₂ - m₄Right.k₂
--- decreasing_by
---   simp_wf
---   have end₂_def : (m₄Right.next k₂_lt_end₂).end₂ = m₄Right.end₂ := by rfl
---   have k₂_def : (m₄Right.next k₂_lt_end₂).k₂ = m₄Right.k₂.succ := by rfl
---   omega
+theorem merge_adjacent_loopLeft_arr_eq
+    [Ord α]
+    {m₄Left : M₄Left α}
+    : (mergeAdjacentChunksIntoAux.loop.loopLeft m₄Left).arr = m₄Left.arr := by
+  unfold mergeAdjacentChunksIntoAux.loop.loopLeft
+  if k₁_lt_start₂ : m₄Left.k₁ < m₄Left.start₂ then
+    simp [k₁_lt_start₂]
+    have := m₄Left.next_arr_eq
+    exact (merge_adjacent_loopLeft_arr_eq (m₄Left := m₄Left.next k₁_lt_start₂))
+  else
+    simp [k₁_lt_start₂]
+    exact (merge_adjacent_loopRight_arr_eq (m₄Right := m₄Left.mkM₄Right k₁_lt_start₂))
+termination_by m₄Left.start₂ - m₄Left.k₁
+decreasing_by
+  simp_wf
+  have start₂_def : (m₄Left.next k₁_lt_start₂).start₂ = m₄Left.start₂ := by rfl
+  have k₁_def : (m₄Left.next k₁_lt_start₂).k₁ = m₄Left.k₁.succ := by rfl
+  omega
 
--- theorem M₂.mkM₄Left_arr_eq
---     [Ord α]
---     {m₂ : M₂ α}
---     {k₁_lt_start₂ : m₂.k₁ < m₂.start₂}
---     : (m₂.mkM₄Left k₁_lt_start₂).arr = m₂.arr := by
---   rfl
+theorem M₂.mkM₄Left_arr_eq
+    [Ord α]
+    {m₂ : M₂ α}
+    : m₂.mkM₄Left.arr = m₂.arr := by
+  rfl
 
--- theorem M₂.mkM₄Right_arr_eq
---     [Ord α]
---     {m₂ : M₂ α}
---     {not_k₁_lt_start₂ : ¬m₂.k₁ < m₂.start₂}
---     : (m₂.mkM₄Right not_k₁_lt_start₂).arr = m₂.arr := by
---   rfl
+theorem M₄Left.mkM₄Right_arr_eq
+    [Ord α]
+    {m₄Left : M₄Left α}
+    {not_k₁_lt_start₂ : ¬m₄Left.k₁ < m₄Left.start₂}
+    : (m₄Left.mkM₄Right not_k₁_lt_start₂).arr = m₄Left.arr := by
+  rfl
 
--- theorem merge_adjacent_loop_arr_eq
---     [Ord α]
---     {m₂ : M₂ α}
---     : (mergeAdjacentChunksIntoAux.loop m₂).arr = m₂.arr := by
---   unfold mergeAdjacentChunksIntoAux.loop
---   if k₁_k₂_in_bounds : m₂.k₁ < m₂.start₂ ∧ m₂.k₂ < m₂.end₂ then
---     simp [k₁_k₂_in_bounds]
---     split
---     . case h_1 =>
---       have : (m₂.mkM₃ k₁_k₂_in_bounds).nextLeft.arr = m₂.arr := by rfl
---       exact (merge_adjacent_loop_arr_eq (m₂ := (m₂.mkM₃ k₁_k₂_in_bounds).nextLeft))
---     . case h_2 =>
---       have : (m₂.mkM₃ k₁_k₂_in_bounds).nextLeft.arr = m₂.arr := by rfl
---       exact (merge_adjacent_loop_arr_eq (m₂ := (m₂.mkM₃ k₁_k₂_in_bounds).nextLeft))
---     . case h_3 =>
---       have : (m₂.mkM₃ k₁_k₂_in_bounds).nextRight.arr = m₂.arr := by rfl
---       exact (merge_adjacent_loop_arr_eq (m₂ := (m₂.mkM₃ k₁_k₂_in_bounds).nextRight))
---   else
---     simp [k₁_k₂_in_bounds]
---     split
---     . case isTrue =>
---         simp [merge_adjacent_loopLeft_arr_eq, M₂.mkM₄Left_arr_eq]
---     . case isFalse =>
---         simp [merge_adjacent_loopRight_arr_eq, M₂.mkM₄Right_arr_eq]
--- termination_by m₂.arr.size - m₂.i
--- decreasing_by
---   all_goals
---     have i_lt_arr_size : m₂.i < m₂.arr.size := by
---       rw [m₂.arr_size_eq_aux_size]
---       exact (m₂.mkM₃ k₁_k₂_in_bounds).i_lt_aux_size
---     exact (Nat.sub_succ_lt_sub_of_lt i_lt_arr_size)
+theorem merge_adjacent_loop_arr_eq
+    [Ord α]
+    {m₂ : M₂ α}
+    : (mergeAdjacentChunksIntoAux.loop m₂).arr = m₂.arr := by
+  unfold mergeAdjacentChunksIntoAux.loop
+  if k₁_k₂_in_bounds : m₂.k₁ < m₂.start₂ ∧ m₂.k₂ < m₂.end₂ then
+    simp [k₁_k₂_in_bounds]
+    split
+    . case h_1 =>
+      have : (m₂.mkM₃ k₁_k₂_in_bounds).nextLeft.arr = m₂.arr := by rfl
+      exact (merge_adjacent_loop_arr_eq (m₂ := (m₂.mkM₃ k₁_k₂_in_bounds).nextLeft))
+    . case h_2 =>
+      have : (m₂.mkM₃ k₁_k₂_in_bounds).nextLeft.arr = m₂.arr := by rfl
+      exact (merge_adjacent_loop_arr_eq (m₂ := (m₂.mkM₃ k₁_k₂_in_bounds).nextLeft))
+    . case h_3 =>
+      have : (m₂.mkM₃ k₁_k₂_in_bounds).nextRight.arr = m₂.arr := by rfl
+      exact (merge_adjacent_loop_arr_eq (m₂ := (m₂.mkM₃ k₁_k₂_in_bounds).nextRight))
+  else
+    simp [k₁_k₂_in_bounds]
+    simp [merge_adjacent_loopLeft_arr_eq, M₂.mkM₄Left_arr_eq]
+    -- split
+    -- . case isTrue =>
+    -- . case isFalse =>
+    --     simp [merge_adjacent_loopRight_arr_eq, M₂.mkM₄Right_arr_eq]
+termination_by m₂.arr.size - m₂.i
+decreasing_by
+  all_goals
+    have i_lt_arr_size : m₂.i < m₂.arr.size := by
+      rw [m₂.arr_size_eq_aux_size]
+      exact (m₂.mkM₃ k₁_k₂_in_bounds).i_lt_aux_size
+    exact (Nat.sub_succ_lt_sub_of_lt i_lt_arr_size)
 
--- theorem merge_adjacent_arr_eq
---     [Ord α]
---     {m₁ : M₁ α}
---     : (mergeAdjacentChunksIntoAux m₁).arr = m₁.arr := by
---   simp [mergeAdjacentChunksIntoAux, merge_adjacent_loop_arr_eq]
+theorem merge_adjacent_arr_eq
+    [Ord α]
+    {m₁ : M₁ α}
+    : (mergeAdjacentChunksIntoAux m₁).arr = m₁.arr := by
+  simp [mergeAdjacentChunksIntoAux, merge_adjacent_loop_arr_eq]
 
--- theorem M₄Left.next_aux_size_eq_arr
---     [Ord α]
---     {m₄Left : M₄Left α}
---     (k₁_lt_start₂ : m₄Left.k₁ < m₄Left.start₂)
---     : (m₄Left.next k₁_lt_start₂).aux.size = m₄Left.arr.size := by
---   simp [M₄Left.next, m₄Left.arr_size_eq_aux_size]
+theorem M₄Right.next_aux_size_eq_arr
+    [Ord α]
+    {m₄Right : M₄Right α}
+    (k₂_lt_end₂ : m₄Right.k₂ < m₄Right.end₂)
+    : (m₄Right.next k₂_lt_end₂).aux.size = m₄Right.arr.size := by
+  simp [M₄Right.next, m₄Right.arr_size_eq_aux_size]
 
--- theorem merge_adjacent_loopLeft_aux_size_eq_arr
---     [Ord α]
---     {m₄Left : M₄Left α}
---     : (mergeAdjacentChunksIntoAux.loop.loopLeft m₄Left).aux.size = m₄Left.arr.size := by
---   unfold mergeAdjacentChunksIntoAux.loop.loopLeft
---   if k₁_lt_start₂ : m₄Left.k₁ < m₄Left.start₂ then
---     simp [k₁_lt_start₂]
---     have := m₄Left.next_arr_eq
---     exact (merge_adjacent_loopLeft_aux_size_eq_arr (m₄Left := m₄Left.next k₁_lt_start₂))
---   else
---     simp [k₁_lt_start₂, m₄Left.arr_size_eq_aux_size]
--- termination_by m₄Left.start₂ - m₄Left.k₁
--- decreasing_by
---   simp_wf
---   have start₂_def : (m₄Left.next k₁_lt_start₂).start₂ = m₄Left.start₂ := by rfl
---   have k₁_def : (m₄Left.next k₁_lt_start₂).k₁ = m₄Left.k₁.succ := by rfl
---   omega
+theorem merge_adjacent_loopRight_aux_size_eq_arr
+    [Ord α]
+    {m₄Right : M₄Right α}
+    : (mergeAdjacentChunksIntoAux.loop.loopLeft.loopRight m₄Right).aux.size = m₄Right.arr.size := by
+  unfold mergeAdjacentChunksIntoAux.loop.loopLeft.loopRight
+  if k₂_lt_end₂ : m₄Right.k₂ < m₄Right.end₂ then
+    simp [k₂_lt_end₂]
+    have := m₄Right.next_arr_eq
+    exact (merge_adjacent_loopRight_aux_size_eq_arr (m₄Right := m₄Right.next k₂_lt_end₂))
+  else
+    simp [k₂_lt_end₂, m₄Right.arr_size_eq_aux_size]
+termination_by m₄Right.end₂ - m₄Right.k₂
+decreasing_by
+  simp_wf
+  have end₂_def : (m₄Right.next k₂_lt_end₂).end₂ = m₄Right.end₂ := by rfl
+  have k₂_def : (m₄Right.next k₂_lt_end₂).k₂ = m₄Right.k₂.succ := by rfl
+  omega
 
--- theorem M₄Right.next_aux_size_eq_arr
---     [Ord α]
---     {m₄Right : M₄Right α}
---     (k₂_lt_end₂ : m₄Right.k₂ < m₄Right.end₂)
---     : (m₄Right.next k₂_lt_end₂).aux.size = m₄Right.arr.size := by
---   simp [M₄Right.next, m₄Right.arr_size_eq_aux_size]
+theorem M₄Left.next_aux_size_eq_arr
+    [Ord α]
+    {m₄Left : M₄Left α}
+    (k₁_lt_start₂ : m₄Left.k₁ < m₄Left.start₂)
+    : (m₄Left.next k₁_lt_start₂).aux.size = m₄Left.arr.size := by
+  simp [M₄Left.next, m₄Left.arr_size_eq_aux_size]
 
--- theorem merge_adjacent_loopRight_aux_size_eq_arr
---     [Ord α]
---     {m₄Right : M₄Right α}
---     : (mergeAdjacentChunksIntoAux.loop.loopRight m₄Right).aux.size = m₄Right.arr.size := by
---   unfold mergeAdjacentChunksIntoAux.loop.loopRight
---   if k₂_lt_end₂ : m₄Right.k₂ < m₄Right.end₂ then
---     simp [k₂_lt_end₂]
---     have := m₄Right.next_arr_eq
---     exact (merge_adjacent_loopRight_aux_size_eq_arr (m₄Right := m₄Right.next k₂_lt_end₂))
---   else
---     simp [k₂_lt_end₂, m₄Right.arr_size_eq_aux_size]
--- termination_by m₄Right.end₂ - m₄Right.k₂
--- decreasing_by
---   simp_wf
---   have end₂_def : (m₄Right.next k₂_lt_end₂).end₂ = m₄Right.end₂ := by rfl
---   have k₂_def : (m₄Right.next k₂_lt_end₂).k₂ = m₄Right.k₂.succ := by rfl
---   omega
+theorem merge_adjacent_loopLeft_aux_size_eq_arr
+    [Ord α]
+    {m₄Left : M₄Left α}
+    : (mergeAdjacentChunksIntoAux.loop.loopLeft m₄Left).aux.size = m₄Left.arr.size := by
+  unfold mergeAdjacentChunksIntoAux.loop.loopLeft
+  if k₁_lt_start₂ : m₄Left.k₁ < m₄Left.start₂ then
+    simp [k₁_lt_start₂]
+    have := m₄Left.next_arr_eq
+    exact (merge_adjacent_loopLeft_aux_size_eq_arr (m₄Left := m₄Left.next k₁_lt_start₂))
+  else
+    simp [k₁_lt_start₂]
+    exact (merge_adjacent_loopRight_aux_size_eq_arr (m₄Right := (m₄Left.mkM₄Right k₁_lt_start₂)))
+termination_by m₄Left.start₂ - m₄Left.k₁
+decreasing_by
+  simp_wf
+  have start₂_def : (m₄Left.next k₁_lt_start₂).start₂ = m₄Left.start₂ := by rfl
+  have k₁_def : (m₄Left.next k₁_lt_start₂).k₁ = m₄Left.k₁.succ := by rfl
+  omega
 
--- theorem merge_adjacent_loop_aux_size_eq_arr
---     [Ord α]
---     {m₂ : M₂ α}
---     : (mergeAdjacentChunksIntoAux.loop m₂).aux.size = m₂.arr.size := by
---   unfold mergeAdjacentChunksIntoAux.loop
---   if k₁_k₂_in_bounds : m₂.k₁ < m₂.start₂ ∧ m₂.k₂ < m₂.end₂ then
---     simp [k₁_k₂_in_bounds]
---     split
---     . case h_1 =>
---       have : (m₂.mkM₃ k₁_k₂_in_bounds).nextLeft.aux.size = m₂.aux.size := by
---         simp [M₂.mkM₃, M₃.nextLeft]
---       exact (merge_adjacent_loop_aux_size_eq_arr (m₂ := (m₂.mkM₃ k₁_k₂_in_bounds).nextLeft))
---     . case h_2 =>
---       have : (m₂.mkM₃ k₁_k₂_in_bounds).nextLeft.aux.size = m₂.aux.size := by
---         simp [M₂.mkM₃, M₃.nextLeft]
---       exact (merge_adjacent_loop_aux_size_eq_arr (m₂ := (m₂.mkM₃ k₁_k₂_in_bounds).nextLeft))
---     . case h_3 =>
---       have : (m₂.mkM₃ k₁_k₂_in_bounds).nextRight.aux.size = m₂.aux.size := by
---         simp [M₂.mkM₃, M₃.nextRight]
---       exact (merge_adjacent_loop_aux_size_eq_arr (m₂ := (m₂.mkM₃ k₁_k₂_in_bounds).nextRight))
---   else
---     simp [k₁_k₂_in_bounds]
---     split
---     . case isTrue =>
---         simp [merge_adjacent_loopLeft_aux_size_eq_arr, M₂.mkM₄Left]
---     . case isFalse =>
---         simp [merge_adjacent_loopRight_aux_size_eq_arr, M₂.mkM₄Right]
--- termination_by m₂.arr.size - m₂.i
--- decreasing_by
---   all_goals
---     have i_lt_arr_size : m₂.i < m₂.arr.size := by
---       rw [m₂.arr_size_eq_aux_size]
---       exact (m₂.mkM₃ k₁_k₂_in_bounds).i_lt_aux_size
---     exact (Nat.sub_succ_lt_sub_of_lt i_lt_arr_size)
+theorem merge_adjacent_loop_aux_size_eq_arr
+    [Ord α]
+    {m₂ : M₂ α}
+    : (mergeAdjacentChunksIntoAux.loop m₂).aux.size = m₂.arr.size := by
+  unfold mergeAdjacentChunksIntoAux.loop
+  if k₁_k₂_in_bounds : m₂.k₁ < m₂.start₂ ∧ m₂.k₂ < m₂.end₂ then
+    simp [k₁_k₂_in_bounds]
+    split
+    . case h_1 =>
+      have : (m₂.mkM₃ k₁_k₂_in_bounds).nextLeft.aux.size = m₂.aux.size := by
+        simp [M₂.mkM₃, M₃.nextLeft]
+      exact (merge_adjacent_loop_aux_size_eq_arr (m₂ := (m₂.mkM₃ k₁_k₂_in_bounds).nextLeft))
+    . case h_2 =>
+      have : (m₂.mkM₃ k₁_k₂_in_bounds).nextLeft.aux.size = m₂.aux.size := by
+        simp [M₂.mkM₃, M₃.nextLeft]
+      exact (merge_adjacent_loop_aux_size_eq_arr (m₂ := (m₂.mkM₃ k₁_k₂_in_bounds).nextLeft))
+    . case h_3 =>
+      have : (m₂.mkM₃ k₁_k₂_in_bounds).nextRight.aux.size = m₂.aux.size := by
+        simp [M₂.mkM₃, M₃.nextRight]
+      exact (merge_adjacent_loop_aux_size_eq_arr (m₂ := (m₂.mkM₃ k₁_k₂_in_bounds).nextRight))
+  else
+    simp [k₁_k₂_in_bounds]
+    exact (merge_adjacent_loopLeft_aux_size_eq_arr (m₄Left := m₂.mkM₄Left))
+termination_by m₂.arr.size - m₂.i
+decreasing_by
+  all_goals
+    have i_lt_arr_size : m₂.i < m₂.arr.size := by
+      rw [m₂.arr_size_eq_aux_size]
+      exact (m₂.mkM₃ k₁_k₂_in_bounds).i_lt_aux_size
+    exact (Nat.sub_succ_lt_sub_of_lt i_lt_arr_size)
 
--- theorem merge_adjacent_aux_size_eq_arr
---     [Ord α]
---     {m₁ : M₁ α}
---     : (mergeAdjacentChunksIntoAux m₁).aux.size = m₁.arr.size := by
---   simp [mergeAdjacentChunksIntoAux, merge_adjacent_loop_aux_size_eq_arr]
+theorem merge_adjacent_aux_size_eq_arr
+    [Ord α]
+    {m₁ : M₁ α}
+    : (mergeAdjacentChunksIntoAux m₁).aux.size = m₁.arr.size := by
+  simp [mergeAdjacentChunksIntoAux, merge_adjacent_loop_aux_size_eq_arr]
 
 structure M₅ (α : Type) where
   arr : Array α
@@ -487,8 +484,7 @@ def M₅.next
     }
   let m₁' : M₁ α := mergeAdjacentChunksIntoAux m₁
   have arr_size_eq_m₁'_aux_size : m₁'.arr.size = m₁'.aux.size := by
-    -- simp [m₁', merge_adjacent_aux_size_eq_arr, merge_adjacent_arr_eq]
-    sorry
+    simp [m₁', merge_adjacent_aux_size_eq_arr, merge_adjacent_arr_eq]
   { arr := m₁'.arr
     aux := m₁'.aux
     size := m₅.size
@@ -548,8 +544,7 @@ def mergeChunksIntoAux
     have : (m₅.next start₁_plus_size_lt_arr_size).arr.size = m₅.arr.size := by
       have : (m₅.next start₁_plus_size_lt_arr_size).arr = m₅.arr := by
         simp [M₅.next]
-        -- exact (merge_adjacent_arr_eq)
-        sorry
+        exact (merge_adjacent_arr_eq)
       simp [*]
     have : (m₅.next start₁_plus_size_lt_arr_size).start₁ = m₅.start₁ + 2 * m₅.size := by
       simp [M₅.next]
@@ -600,8 +595,7 @@ theorem mergeChunksIntoAux.loop_size_eq_arr_size
     simp [start₁_plus_size_lt_arr_size]
     have : (m₅.next start₁_plus_size_lt_arr_size).arr.size = m₅.arr.size := by
       have : (m₅.next start₁_plus_size_lt_arr_size).arr = m₅.arr := by
-        -- simp [M₅.next, merge_adjacent_arr_eq]
-        sorry
+        simp [M₅.next, merge_adjacent_arr_eq]
       simp [*]
     simp [
       mergeChunksIntoAux.loop_size_eq_arr_size
@@ -617,8 +611,7 @@ termination_by m₅.arr.size - m₅.start₁
 decreasing_by
   simp_wf
   have : (m₅.next start₁_plus_size_lt_arr_size).arr = m₅.arr := by
-    -- simp [M₅.next, merge_adjacent_arr_eq]
-    sorry
+    simp [M₅.next, merge_adjacent_arr_eq]
   have : (m₅.next start₁_plus_size_lt_arr_size).start₁ = m₅.start₁ + 2 * m₅.size := by
     simp [M₅.next]
   have := m₅.size_gt_0
